Adapt proofs for latest summary versions

EvmEquivalence/Equivalence/Push0Equivalence.lean
@@ -14,7 +14,6 @@ namespace Push0Equivalence
 
 def push0LHS
   {GAS_CELL PC_CELL : SortInt}
-  {K_CELL : SortK}
   {SCHEDULE_CELL : SortSchedule}
   {USEGAS_CELL : SortBool}
   {WS : SortWordStack}
@@ -43,9 +42,10 @@ def push0LHS
   {_Gen6 : SortLocalMemCell}
   {_Gen7 : SortMemoryUsedCell}
   {_Gen8 : SortCallGasCell}
-  {_Gen9 : SortStaticCell}: SortGeneratedTopCell :=
+  {_Gen9 : SortStaticCell}
+  {_K_CELL : SortK} : SortGeneratedTopCell :=
   { kevm := {
-      k := { val := SortK.kseq ((@inj SortInternalOp SortKItem) (SortInternalOp.«#next[_]_EVM_InternalOp_MaybeOpCode» ((@inj SortPushOp SortMaybeOpCode) SortPushOp.PUSHZERO_EVM_PushOp))) K_CELL },
+      k := { val := SortK.kseq ((@inj SortInternalOp SortKItem) (SortInternalOp.«#next[_]_EVM_InternalOp_MaybeOpCode» ((@inj SortPushOp SortMaybeOpCode) SortPushOp.PUSHZERO_EVM_PushOp))) _K_CELL },
       exitCode := _Gen22,
       mode := _Gen23,
       schedule := { val := SCHEDULE_CELL },
@@ -82,78 +82,8 @@ def push0LHS
     generatedCounter := _DotVar0 }
 
 def push0RHS
-  {_Val11 _Val13 : SortInt}
-  {K_CELL : SortK}
+  {_Val6 _Val8 : SortInt}
   {SCHEDULE_CELL : SortSchedule}
-  {WS : SortWordStack}
-  {_DotVar0 : SortGeneratedCounterCell}
-  {_DotVar2 : SortNetworkCell}
-  {_Gen0 : SortProgramCell}
-  {_Gen1 : SortJumpDestsCell}
-  {_Gen10 : SortCallDepthCell}
-  {_Gen11 : SortOutputCell}
-  {_Gen12 : SortStatusCodeCell}
-  {_Gen13 : SortCallStackCell}
-  {_Gen14 : SortInterimStatesCell}
-  {_Gen15 : SortTouchedAccountsCell}
-  {_Gen16 : SortVersionedHashesCell}
-  {_Gen17 : SortSubstateCell}
-  {_Gen18 : SortGasPriceCell}
-  {_Gen19 : SortOriginCell}
-  {_Gen2 : SortIdCell}
-  {_Gen20 : SortBlockhashesCell}
-  {_Gen21 : SortBlockCell}
-  {_Gen22 : SortExitCodeCell}
-  {_Gen23 : SortModeCell}
-  {_Gen3 : SortCallerCell}
-  {_Gen4 : SortCallDataCell}
-  {_Gen5 : SortCallValueCell}
-  {_Gen6 : SortLocalMemCell}
-  {_Gen7 : SortMemoryUsedCell}
-  {_Gen8 : SortCallGasCell}
-  {_Gen9 : SortStaticCell}: SortGeneratedTopCell :=
-  { kevm := {
-      k := { val := K_CELL },
-      exitCode := _Gen22,
-      mode := _Gen23,
-      schedule := { val := SCHEDULE_CELL },
-      useGas := { val := true },
-      ethereum := {
-        evm := {
-          output := _Gen11,
-          statusCode := _Gen12,
-          callStack := _Gen13,
-          interimStates := _Gen14,
-          touchedAccounts := _Gen15,
-          callState := {
-            program := _Gen0,
-            jumpDests := _Gen1,
-            id := _Gen2,
-            caller := _Gen3,
-            callData := _Gen4,
-            callValue := _Gen5,
-            wordStack := { val := SortWordStack.«_:__EVM-TYPES_WordStack_Int_WordStack» 0 WS },
-            localMem := _Gen6,
-            pc := { val := _Val11 },
-            gas := { val := (@inj SortInt SortGas) _Val13 },
-            memoryUsed := _Gen7,
-            callGas := _Gen8,
-            static := _Gen9,
-            callDepth := _Gen10 },
-          versionedHashes := _Gen16,
-          substate := _Gen17,
-          gasPrice := _Gen18,
-          origin := _Gen19,
-          blockhashes := _Gen20,
-          block := _Gen21 },
-        network := _DotVar2 } },
-    generatedCounter := _DotVar0 }
-
-theorem rw_push0LHS_push0RHS
-  {GAS_CELL PC_CELL _Val0 _Val11 _Val12 _Val13 _Val3 _Val6 : SortInt}
-  {K_CELL : SortK}
-  {SCHEDULE_CELL : SortSchedule}
-  {USEGAS_CELL _Val1 _Val10 _Val2 _Val4 _Val5 _Val7 _Val8 _Val9 : SortBool}
   {WS : SortWordStack}
   {_DotVar0 : SortGeneratedCounterCell}
   {_DotVar2 : SortNetworkCell}
@@ -181,30 +111,95 @@ theorem rw_push0LHS_push0RHS
   {_Gen7 : SortMemoryUsedCell}
   {_Gen8 : SortCallGasCell}
   {_Gen9 : SortStaticCell}
-  (defn_Val0 : «_<_>_SCHEDULE_Int_ScheduleConst_Schedule» SortScheduleConst.Gbase_SCHEDULE_ScheduleConst SCHEDULE_CELL = some _Val0)
-  (defn_Val1 : «_<=Int_» _Val0 GAS_CELL = some _Val1)
-  (defn_Val2 : _andBool_ USEGAS_CELL _Val1 = some _Val2)
-  (defn_Val3 : sizeWordStackAux WS 0 = some _Val3)
-  (defn_Val4 : «_<Int_» _Val3 0 = some _Val4)
-  (defn_Val5 : notBool_ _Val4 = some _Val5)
-  (defn_Val6 : sizeWordStackAux WS 0 = some _Val6)
-  (defn_Val7 : «_<Int_» 1023 _Val6 = some _Val7)
-  (defn_Val8 : notBool_ _Val7 = some _Val8)
-  (defn_Val9 : _andBool_ _Val5 _Val8 = some _Val9)
-  (defn_Val10 : _andBool_ _Val2 _Val9 = some _Val10)
-  (defn_Val11 : «_+Int_» PC_CELL 1 = some _Val11)
-  (defn_Val12 : «_<_>_SCHEDULE_Int_ScheduleConst_Schedule» SortScheduleConst.Gbase_SCHEDULE_ScheduleConst SCHEDULE_CELL = some _Val12)
-  (defn_Val13 : «_-Int_» GAS_CELL _Val12 = some _Val13)
-  (req : _Val10 = true) :
+  {_K_CELL : SortK} : SortGeneratedTopCell :=
+  { kevm := {
+      k := { val := _K_CELL },
+      exitCode := _Gen22,
+      mode := _Gen23,
+      schedule := { val := SCHEDULE_CELL },
+      useGas := { val := true },
+      ethereum := {
+        evm := {
+          output := _Gen11,
+          statusCode := _Gen12,
+          callStack := _Gen13,
+          interimStates := _Gen14,
+          touchedAccounts := _Gen15,
+          callState := {
+            program := _Gen0,
+            jumpDests := _Gen1,
+            id := _Gen2,
+            caller := _Gen3,
+            callData := _Gen4,
+            callValue := _Gen5,
+            wordStack := { val := SortWordStack.«_:__EVM-TYPES_WordStack_Int_WordStack» 0 WS },
+            localMem := _Gen6,
+            pc := { val := _Val6 },
+            gas := { val := (@inj SortInt SortGas) _Val8 },
+            memoryUsed := _Gen7,
+            callGas := _Gen8,
+            static := _Gen9,
+            callDepth := _Gen10 },
+          versionedHashes := _Gen16,
+          substate := _Gen17,
+          gasPrice := _Gen18,
+          origin := _Gen19,
+          blockhashes := _Gen20,
+          block := _Gen21 },
+        network := _DotVar2 } },
+    generatedCounter := _DotVar0 }
+
+theorem rw_push0LHS_push0RHS
+  {GAS_CELL PC_CELL _Val0 _Val2 _Val6 _Val7 _Val8 : SortInt}
+  {SCHEDULE_CELL : SortSchedule}
+  {USEGAS_CELL _Val1 _Val3 _Val4 _Val5 : SortBool}
+  {WS : SortWordStack}
+  {_DotVar0 : SortGeneratedCounterCell}
+  {_DotVar2 : SortNetworkCell}
+  {_Gen0 : SortProgramCell}
+  {_Gen1 : SortJumpDestsCell}
+  {_Gen10 : SortCallDepthCell}
+  {_Gen11 : SortOutputCell}
+  {_Gen12 : SortStatusCodeCell}
+  {_Gen13 : SortCallStackCell}
+  {_Gen14 : SortInterimStatesCell}
+  {_Gen15 : SortTouchedAccountsCell}
+  {_Gen16 : SortVersionedHashesCell}
+  {_Gen17 : SortSubstateCell}
+  {_Gen18 : SortGasPriceCell}
+  {_Gen19 : SortOriginCell}
+  {_Gen2 : SortIdCell}
+  {_Gen20 : SortBlockhashesCell}
+  {_Gen21 : SortBlockCell}
+  {_Gen22 : SortExitCodeCell}
+  {_Gen23 : SortModeCell}
+  {_Gen3 : SortCallerCell}
+  {_Gen4 : SortCallDataCell}
+  {_Gen5 : SortCallValueCell}
+  {_Gen6 : SortLocalMemCell}
+  {_Gen7 : SortMemoryUsedCell}
+  {_Gen8 : SortCallGasCell}
+  {_Gen9 : SortStaticCell}
+  {_K_CELL : SortK}
+  (defn_Val0 : sizeWordStackAux WS 0 = some _Val0)
+  (defn_Val1 : «_<=Int_» _Val0 1023 = some _Val1)
+  (defn_Val2 : «_<_>_SCHEDULE_Int_ScheduleConst_Schedule» SortScheduleConst.Gbase_SCHEDULE_ScheduleConst SCHEDULE_CELL = some _Val2)
+  (defn_Val3 : «_<=Int_» _Val2 GAS_CELL = some _Val3)
+  (defn_Val4 : _andBool_ _Val1 _Val3 = some _Val4)
+  (defn_Val5 : _andBool_ USEGAS_CELL _Val4 = some _Val5)
+  (defn_Val6 : «_+Int_» PC_CELL 1 = some _Val6)
+  (defn_Val7 : «_<_>_SCHEDULE_Int_ScheduleConst_Schedule» SortScheduleConst.Gbase_SCHEDULE_ScheduleConst SCHEDULE_CELL = some _Val7)
+  (defn_Val8 : «_-Int_» GAS_CELL _Val7 = some _Val8)
+  (req : _Val5 = true) :
   Rewrites
-  (@push0LHS GAS_CELL PC_CELL K_CELL SCHEDULE_CELL USEGAS_CELL WS _DotVar0 _DotVar2 _Gen0 _Gen1 _Gen10 _Gen11 _Gen12 _Gen13 _Gen14 _Gen15 _Gen16 _Gen17 _Gen18 _Gen19 _Gen2 _Gen20 _Gen21 _Gen22 _Gen23 _Gen3 _Gen4 _Gen5 _Gen6 _Gen7 _Gen8 _Gen9)
-  (@push0RHS _Val11 _Val13 K_CELL SCHEDULE_CELL WS _DotVar0 _DotVar2 _Gen0 _Gen1 _Gen10 _Gen11 _Gen12 _Gen13 _Gen14 _Gen15 _Gen16 _Gen17 _Gen18 _Gen19 _Gen2 _Gen20 _Gen21 _Gen22 _Gen23 _Gen3 _Gen4 _Gen5 _Gen6 _Gen7 _Gen8 _Gen9) :=
-  by apply Rewrites.PUSHZERO_SUMMARY_PUSHZERO_SUMMARY_1 <;> try assumption
-     all_goals simp_all [notBool_def, andBool_def]
+  (@push0LHS GAS_CELL PC_CELL SCHEDULE_CELL USEGAS_CELL WS _DotVar0 _DotVar2 _Gen0 _Gen1 _Gen10 _Gen11 _Gen12 _Gen13 _Gen14 _Gen15 _Gen16 _Gen17 _Gen18 _Gen19 _Gen2 _Gen20 _Gen21 _Gen22 _Gen23 _Gen3 _Gen4 _Gen5 _Gen6 _Gen7 _Gen8 _Gen9 _K_CELL)
+  (@push0RHS _Val6 _Val8 SCHEDULE_CELL WS _DotVar0 _DotVar2 _Gen0 _Gen1 _Gen10 _Gen11 _Gen12 _Gen13 _Gen14 _Gen15 _Gen16 _Gen17 _Gen18 _Gen19 _Gen2 _Gen20 _Gen21 _Gen22 _Gen23 _Gen3 _Gen4 _Gen5 _Gen6 _Gen7 _Gen8 _Gen9 _K_CELL) :=
+  by
+    apply Rewrites.PUSHZERO_SUMMARY_PUSHZERO_SUMMARY_USEGAS <;> try assumption
+    all_goals simp_all [notBool_def, andBool_def]
 
 theorem push0_prestate_equiv
   {GAS_CELL PC_CELL : SortInt}
-  {K_CELL : SortK}
   {SCHEDULE_CELL : SortSchedule}
   {USEGAS_CELL : SortBool}
   {WS : SortWordStack}
@@ -234,8 +229,9 @@ theorem push0_prestate_equiv
   {_Gen7 : SortMemoryUsedCell}
   {_Gen8 : SortCallGasCell}
   {_Gen9 : SortStaticCell}
+  {_K_CELL : SortK}
   {symState : EVM.State}:
-  let lhs := (@push0LHS GAS_CELL PC_CELL K_CELL SCHEDULE_CELL USEGAS_CELL WS _DotVar0 _DotVar2 _Gen0 _Gen1 _Gen10 _Gen11 _Gen12 _Gen13 _Gen14 _Gen15 _Gen16 _Gen17 _Gen18 _Gen19 _Gen2 _Gen20 _Gen21 _Gen22 _Gen23 _Gen3 _Gen4 _Gen5 _Gen6 _Gen7 _Gen8 _Gen9)
+  let lhs := (@push0LHS GAS_CELL PC_CELL SCHEDULE_CELL USEGAS_CELL WS _DotVar0 _DotVar2 _Gen0 _Gen1 _Gen10 _Gen11 _Gen12 _Gen13 _Gen14 _Gen15 _Gen16 _Gen17 _Gen18 _Gen19 _Gen2 _Gen20 _Gen21 _Gen22 _Gen23 _Gen3 _Gen4 _Gen5 _Gen6 _Gen7 _Gen8 _Gen9 _K_CELL)
   stateMap symState lhs =
   {symState with
     stack := wordStackMap WS
@@ -254,9 +250,7 @@ theorem push0_prestate_equiv
     } := rfl
 
 theorem push0_poststate_equiv
-  (PC_CELL : SortInt)
-  {_Val11 _Val13 : SortInt}
-  {K_CELL : SortK}
+  {PC_CELL _Val6 _Val8 : SortInt}
   {SCHEDULE_CELL : SortSchedule}
   {WS : SortWordStack}
   {_DotVar0 : SortGeneratedCounterCell}
@@ -285,14 +279,15 @@ theorem push0_poststate_equiv
   {_Gen7 : SortMemoryUsedCell}
   {_Gen8 : SortCallGasCell}
   {_Gen9 : SortStaticCell}
+  {_K_CELL : SortK}
   {symState : EVM.State}
-  (defn_Val11 : «_+Int_» PC_CELL 1 = some _Val11):
-  let rhs := (@push0RHS _Val11 _Val13 K_CELL SCHEDULE_CELL WS _DotVar0 _DotVar2 _Gen0 _Gen1 _Gen10 _Gen11 _Gen12 _Gen13 _Gen14 _Gen15 _Gen16 _Gen17 _Gen18 _Gen19 _Gen2 _Gen20 _Gen21 _Gen22 _Gen23 _Gen3 _Gen4 _Gen5 _Gen6 _Gen7 _Gen8 _Gen9)
+  (defn_Val11 : «_+Int_» PC_CELL 1 = some _Val6):
+  let rhs := (@push0RHS _Val6 _Val8 SCHEDULE_CELL WS _DotVar0 _DotVar2 _Gen0 _Gen1 _Gen10 _Gen11 _Gen12 _Gen13 _Gen14 _Gen15 _Gen16 _Gen17 _Gen18 _Gen19 _Gen2 _Gen20 _Gen21 _Gen22 _Gen23 _Gen3 _Gen4 _Gen5 _Gen6 _Gen7 _Gen8 _Gen9 _K_CELL)
   stateMap symState rhs =
   {symState with
     stack := .ofNat 0 :: wordStackMap WS
     pc := intMap («_+Int'_» PC_CELL 1)
-    gasAvailable := intMap _Val13
+    gasAvailable := intMap _Val8
     executionEnv := {symState.executionEnv with
                   code := _Gen0.val,
                   codeOwner := idMap rhs.Iₐ,
@@ -306,10 +301,9 @@ theorem push0_poststate_equiv
     } := by aesop (add simp [«_+Int'_»])
 
 theorem step_push0_equiv
-  {GAS_CELL PC_CELL _Val0 _Val11 _Val12 _Val13 _Val3 _Val6 : SortInt}
-  {K_CELL : SortK}
+  {GAS_CELL PC_CELL _Val0 _Val2 _Val6 _Val7 _Val8 : SortInt}
   {SCHEDULE_CELL : SortSchedule}
-  {USEGAS_CELL _Val1 _Val10 _Val2 _Val4 _Val5 _Val7 _Val8 _Val9 : SortBool}
+  {USEGAS_CELL _Val1 _Val3 _Val4 _Val5 : SortBool}
   {WS : SortWordStack}
   {_DotVar0 : SortGeneratedCounterCell}
   {_DotVar2 : SortNetworkCell}
@@ -337,21 +331,17 @@ theorem step_push0_equiv
   {_Gen7 : SortMemoryUsedCell}
   {_Gen8 : SortCallGasCell}
   {_Gen9 : SortStaticCell}
-  (defn_Val0 : «_<_>_SCHEDULE_Int_ScheduleConst_Schedule» SortScheduleConst.Gbase_SCHEDULE_ScheduleConst SCHEDULE_CELL = some _Val0)
-  (defn_Val1 : «_<=Int_» _Val0 GAS_CELL = some _Val1)
-  /- (defn_Val2 : _andBool_ USEGAS_CELL _Val1 = some _Val2) -/
-  (defn_Val3 : sizeWordStackAux WS 0 = some _Val3)
-  (defn_Val4 : «_<Int_» _Val3 0 = some _Val4)
-  /- (defn_Val5 : notBool_ _Val4 = some _Val5) -/
-  (defn_Val6 : sizeWordStackAux WS 0 = some _Val6)
-  (defn_Val7 : «_<Int_» 1023 _Val6 = some _Val7)
-  /- (defn_Val8 : notBool_ _Val7 = some _Val8)
-  (defn_Val9 : _andBool_ _Val5 _Val8 = some _Val9) -/
-  (defn_Val10 : _andBool_ _Val2 _Val9 = some _Val10)
-  (defn_Val11 : «_+Int_» PC_CELL 1 = some _Val11)
-  (defn_Val12 : «_<_>_SCHEDULE_Int_ScheduleConst_Schedule» SortScheduleConst.Gbase_SCHEDULE_ScheduleConst SCHEDULE_CELL = some _Val12)
-  (defn_Val13 : «_-Int_» GAS_CELL _Val12 = some _Val13)
-  (req : _Val10 = true)
+  {_K_CELL : SortK}
+  /- (defn_Val0 : sizeWordStackAux WS 0 = some _Val0)
+  (defn_Val1 : «_<=Int_» _Val0 1023 = some _Val1) -/
+  (defn_Val2 : «_<_>_SCHEDULE_Int_ScheduleConst_Schedule» SortScheduleConst.Gbase_SCHEDULE_ScheduleConst SCHEDULE_CELL = some _Val2)
+  (defn_Val3 : «_<=Int_» _Val2 GAS_CELL = some _Val3)
+  /- (defn_Val4 : _andBool_ _Val1 _Val3 = some _Val4) -/
+  (defn_Val5 : _andBool_ USEGAS_CELL _Val4 = some _Val5)
+  (defn_Val6 : «_+Int_» PC_CELL 1 = some _Val6)
+  (defn_Val7 : «_<_>_SCHEDULE_Int_ScheduleConst_Schedule» SortScheduleConst.Gbase_SCHEDULE_ScheduleConst SCHEDULE_CELL = some _Val7)
+  (defn_Val8 : «_-Int_» GAS_CELL _Val7 = some _Val8)
+  (req : _Val5 = true)
   (symState : EVM.State)
   -- needed for EVM.step
   (gas gasCost : ℕ)
@@ -363,23 +353,21 @@ theorem step_push0_equiv
   (gasCostValue : gasCost = GasConstants.Gbase)
   (pcountSmall : PC_CELL + 1 < UInt256.size)
   (pcountNonneg : 0 ≤ PC_CELL):
-  EVM.step_push0 gas gasCost (stateMap symState (@push0LHS GAS_CELL PC_CELL K_CELL SCHEDULE_CELL USEGAS_CELL WS _DotVar0 _DotVar2 _Gen0 _Gen1 _Gen10 _Gen11 _Gen12 _Gen13 _Gen14 _Gen15 _Gen16 _Gen17 _Gen18 _Gen19 _Gen2 _Gen20 _Gen21 _Gen22 _Gen23 _Gen3 _Gen4 _Gen5 _Gen6 _Gen7 _Gen8 _Gen9)) =
-  .ok (stateMap {symState with execLength := symState.execLength + 1} (@push0RHS _Val11 _Val13 K_CELL SCHEDULE_CELL WS _DotVar0 _DotVar2 _Gen0 _Gen1 _Gen10 _Gen11 _Gen12 _Gen13 _Gen14 _Gen15 _Gen16 _Gen17 _Gen18 _Gen19 _Gen2 _Gen20 _Gen21 _Gen22 _Gen23 _Gen3 _Gen4 _Gen5 _Gen6 _Gen7 _Gen8 _Gen9)) := by
-  rw [push0_prestate_equiv, (push0_poststate_equiv PC_CELL)]
+  EVM.step_push0 gas gasCost (stateMap symState (@push0LHS GAS_CELL PC_CELL SCHEDULE_CELL USEGAS_CELL WS _DotVar0 _DotVar2 _Gen0 _Gen1 _Gen10 _Gen11 _Gen12 _Gen13 _Gen14 _Gen15 _Gen16 _Gen17 _Gen18 _Gen19 _Gen2 _Gen20 _Gen21 _Gen22 _Gen23 _Gen3 _Gen4 _Gen5 _Gen6 _Gen7 _Gen8 _Gen9 _K_CELL)) =
+  .ok (stateMap {symState with execLength := symState.execLength + 1} (@push0RHS _Val6 _Val8 SCHEDULE_CELL WS _DotVar0 _DotVar2 _Gen0 _Gen1 _Gen10 _Gen11 _Gen12 _Gen13 _Gen14 _Gen15 _Gen16 _Gen17 _Gen18 _Gen19 _Gen2 _Gen20 _Gen21 _Gen22 _Gen23 _Gen3 _Gen4 _Gen5 _Gen6 _Gen7 _Gen8 _Gen9 _K_CELL)) := by
+  rw [push0_prestate_equiv, (push0_poststate_equiv defn_Val6)]
   cases gas; contradiction
   rw [EVM.step_push0_summary] <;> try assumption
   simp [push0LHS, push0RHS]; constructor <;> try constructor
   . aesop (add simp [GasConstants.Gbase, «_-Int_», cancun_def, intMap_sub_dist])
   . rw [plusInt_def, ←UInt256.add_succ_mod_size, intMap_add_dist] <;> aesop
-  . aesop (add simp [«_+Int_»])
 
 attribute [local simp] GasConstants.Gbase
 
 theorem X_push0_equiv
-  {GAS_CELL PC_CELL _Val0 _Val11 _Val12 _Val13 _Val3 _Val6 : SortInt}
-  {K_CELL : SortK}
+  {GAS_CELL PC_CELL _Val0 _Val2 _Val6 _Val7 _Val8 : SortInt}
   {SCHEDULE_CELL : SortSchedule}
-  {USEGAS_CELL _Val1 _Val10 _Val2 _Val4 _Val5 _Val7 _Val8 _Val9 : SortBool}
+  {USEGAS_CELL _Val1 _Val3 _Val4 _Val5 : SortBool}
   {WS : SortWordStack}
   {_DotVar0 : SortGeneratedCounterCell}
   {_DotVar2 : SortNetworkCell}
@@ -407,21 +395,17 @@ theorem X_push0_equiv
   {_Gen7 : SortMemoryUsedCell}
   {_Gen8 : SortCallGasCell}
   {_Gen9 : SortStaticCell}
-  (defn_Val0 : «_<_>_SCHEDULE_Int_ScheduleConst_Schedule» SortScheduleConst.Gbase_SCHEDULE_ScheduleConst SCHEDULE_CELL = some _Val0)
-  (defn_Val1 : «_<=Int_» _Val0 GAS_CELL = some _Val1)
-  (defn_Val2 : _andBool_ USEGAS_CELL _Val1 = some _Val2)
-  (defn_Val3 : sizeWordStackAux WS 0 = some _Val3)
-  (defn_Val4 : «_<Int_» _Val3 0 = some _Val4)
-  --(defn_Val5 : notBool_ _Val4 = some _Val5)
-  (defn_Val6 : sizeWordStackAux WS 0 = some _Val6)
-  (defn_Val7 : «_<Int_» 1023 _Val6 = some _Val7)
-  (defn_Val8 : notBool_ _Val7 = some _Val8)
-  (defn_Val9 : _andBool_ _Val5 _Val8 = some _Val9)
-  (defn_Val10 : _andBool_ _Val2 _Val9 = some _Val10)
-  (defn_Val11 : «_+Int_» PC_CELL 1 = some _Val11)
-  (defn_Val12 : «_<_>_SCHEDULE_Int_ScheduleConst_Schedule» SortScheduleConst.Gbase_SCHEDULE_ScheduleConst SCHEDULE_CELL = some _Val12)
-  (defn_Val13 : «_-Int_» GAS_CELL _Val12 = some _Val13)
-  (req : _Val10 = true)
+  {_K_CELL : SortK}
+  (defn_Val0 : sizeWordStackAux WS 0 = some _Val0)
+  (defn_Val1 : «_<=Int_» _Val0 1023 = some _Val1)
+  (defn_Val2 : «_<_>_SCHEDULE_Int_ScheduleConst_Schedule» SortScheduleConst.Gbase_SCHEDULE_ScheduleConst SCHEDULE_CELL = some _Val2)
+  (defn_Val3 : «_<=Int_» _Val2 GAS_CELL = some _Val3)
+  (defn_Val4 : _andBool_ _Val1 _Val3 = some _Val4)
+  (defn_Val5 : _andBool_ USEGAS_CELL _Val4 = some _Val5)
+  (defn_Val6 : «_+Int_» PC_CELL 1 = some _Val6)
+  (defn_Val7 : «_<_>_SCHEDULE_Int_ScheduleConst_Schedule» SortScheduleConst.Gbase_SCHEDULE_ScheduleConst SCHEDULE_CELL = some _Val7)
+  (defn_Val8 : «_-Int_» GAS_CELL _Val7 = some _Val8)
+  (req : _Val5 = true)
   (symState : EVM.State)
   -- Necessary assumptions for equivalence
   (cancun : SCHEDULE_CELL = .CANCUN_EVM)
@@ -434,9 +418,9 @@ theorem X_push0_equiv
   (codePush0 : _Gen0 = ⟨⟨#[(0x5F : UInt8)]⟩⟩)
   (pcZero : PC_CELL = 0)
   (returnEmpty : _Gen11 = ⟨ByteArray.empty⟩):
-  EVM.X false (UInt256.toNat (intMap GAS_CELL)) (stateMap symState (@push0LHS GAS_CELL PC_CELL K_CELL SCHEDULE_CELL USEGAS_CELL WS _DotVar0 _DotVar2 _Gen0 _Gen1 _Gen10 _Gen11 _Gen12 _Gen13 _Gen14 _Gen15 _Gen16 _Gen17 _Gen18 _Gen19 _Gen2 _Gen20 _Gen21 _Gen22 _Gen23 _Gen3 _Gen4 _Gen5 _Gen6 _Gen7 _Gen8 _Gen9)) =
-  .ok (.success (stateMap {symState with execLength := symState.execLength + 2} (@push0RHS _Val11 _Val13 K_CELL SCHEDULE_CELL WS _DotVar0 _DotVar2 _Gen0 _Gen1 _Gen10 _Gen11 _Gen12 _Gen13 _Gen14 _Gen15 _Gen16 _Gen17 _Gen18 _Gen19 _Gen2 _Gen20 _Gen21 _Gen22 _Gen23 _Gen3 _Gen4 _Gen5 _Gen6 _Gen7 _Gen8 _Gen9)) ByteArray.empty) := by
-  rw [codePush0, pcZero, push0_prestate_equiv, (push0_poststate_equiv PC_CELL)] <;> try assumption
+  EVM.X false (UInt256.toNat (intMap GAS_CELL)) (stateMap symState (@push0LHS GAS_CELL PC_CELL SCHEDULE_CELL USEGAS_CELL WS _DotVar0 _DotVar2 _Gen0 _Gen1 _Gen10 _Gen11 _Gen12 _Gen13 _Gen14 _Gen15 _Gen16 _Gen17 _Gen18 _Gen19 _Gen2 _Gen20 _Gen21 _Gen22 _Gen23 _Gen3 _Gen4 _Gen5 _Gen6 _Gen7 _Gen8 _Gen9 _K_CELL)) =
+  .ok (.success (stateMap {symState with execLength := symState.execLength + 2} (@push0RHS _Val6 _Val8 SCHEDULE_CELL WS _DotVar0 _DotVar2 _Gen0 _Gen1 _Gen10 _Gen11 _Gen12 _Gen13 _Gen14 _Gen15 _Gen16 _Gen17 _Gen18 _Gen19 _Gen2 _Gen20 _Gen21 _Gen22 _Gen23 _Gen3 _Gen4 _Gen5 _Gen6 _Gen7 _Gen8 _Gen9 _K_CELL)) ByteArray.empty) := by
+  rw [codePush0, pcZero, push0_prestate_equiv, (push0_poststate_equiv defn_Val6)] <;> try assumption
   rw [intMap_toNat] <;> first | linarith | try assumption
   cases cgc: (UInt256.toNat (intMap GAS_CELL))
   . rw [intMap_toNat, Int.toNat_eq_zero] at cgc <;> linarith
@@ -445,8 +429,7 @@ theorem X_push0_equiv
     . aesop (add simp [«_-Int_», intMap_sub_dist, push0LHS, push0RHS])
       (add safe (by rw [intMap_sub_dist])) (add safe (by linarith))
     . rw [intMap_toNat] <;> aesop (add safe (by linarith))
-    . simp [defn_Val3] at defn_Val6; subst defn_Val6
-      aesop (add simp [sizeWordStack_def, andBool_def, notBool_def,  ltInt_def])
+    . aesop (add simp [sizeWordStack_def, andBool_def, notBool_def, «_<=Int_»])
       (add safe (by linarith))
 
 end Push0Equivalence
