EvmEquivalence/Equivalence/AddEquivalence.lean
@@ -192,7 +192,7 @@ theorem rw_addLHS_addRHS
   Rewrites
   (@addLHS GAS_CELL PC_CELL W0 W1 K_CELL SCHEDULE_CELL USEGAS_CELL WS _DotVar0 _DotVar2 _Gen0 _Gen1 _Gen10 _Gen11 _Gen12 _Gen13 _Gen14 _Gen15 _Gen16 _Gen17 _Gen18 _Gen19 _Gen2 _Gen20 _Gen21 _Gen22 _Gen23 _Gen3 _Gen4 _Gen5 _Gen6 _Gen7 _Gen8 _Gen9)
   (@addRHS _Val0 _Val3 _Val4 _Val5 _Val6 _Val7 K_CELL SCHEDULE_CELL _Val1 _Val2 WS _DotVar0 _DotVar2 _Gen0 _Gen1 _Gen10 _Gen11 _Gen12 _Gen13 _Gen14 _Gen15 _Gen16 _Gen17 _Gen18 _Gen19 _Gen2 _Gen20 _Gen21 _Gen22 _Gen23 _Gen3 _Gen4 _Gen5 _Gen6 _Gen7 _Gen8 _Gen9) := by
-  apply Rewrites.ADD_SUMMARY_ADD_SUMMARY_0 <;> try assumption
+  apply Rewrites.ADD_SUMMARY_ADD_SUMMARY_USEGAS <;> try assumption
   simp_all
 
 theorem add_prestate_equiv
